more on add with carry case N=1 proof

test/lean/Proofs.lean
@@ -1,4 +1,5 @@
 import Test.Funs
+import Base
 
 open Primitives
 open Result
@@ -8,36 +9,70 @@ namespace test
 
 namespace arithmetics
 
-def BigInt.valImpl (l : List U64) : Int :=
-  match l with
-  | a::b => a.val + (valImpl b) * (2 ^ 64)
-  | [] => 0
+def BigInt.valImpl [Inhabited U64] (l : List U64) : Int :=
+  if l.len = 0
+  then 0
+  else (l.index 0) + (valImpl (l.idrop 1)) * (2 ^ 64)
+termination_by BigInt.valImpl l => l.len.toNat
+decreasing_by
+  simp_wf
+  have : 1 ≤ l.len := by scalar_tac
+  simp [Int.toNat_sub_of_le, *]
+  sorry
 
-def BigInt.val {N : Usize} (x : BigInt N) : Int := valImpl x.num.val
 
-def BigInt.max_value (N : Usize) : Int := (U64.max + 1) ^ (Int.toNat N.val) - 1
+-- def BigInt.valImpl (l : List U64) : Int :=
+--   match l with
+--   | a::b => a.val + (valImpl b) * (2 ^ 64)
+--   | [] => 0
+
+def BigInt.val {N : Usize} [Inhabited U64] (x : BigInt N) : Int := valImpl x.num.val
+
+def BigInt.max_value [Inhabited U64] (N : Usize) : Int := (U64.max + 1) ^ (Int.toNat N.val) - 1
+
+lemma tmp: 
+  ∀ (N : Usize) (self : arithmetics.BigInt N),
+  self.num.val.len = N.val := by intro N; intro self; simp [List.len_eq_length]; sorry
 
 theorem adc_for_add_with_carry_spec (a : U64) (b : U64) (carry : U8) :
-  match adc_for_add_with_carry a b carry with
-  | ret new_carry => new_carry = (a.val + b.val + carry.val) / (2 ^ 64)
-  | _ => ⊥
-  := by sorry
+  ∃ new_carry, adc_for_add_with_carry a b carry = .ret new_carry ∧ 
+  new_carry = (a.val + b.val + carry.val) / (2 ^ 64) := by sorry
 
 theorem adc_for_add_with_carry_back_spec (a : U64) (b : U64) (carry : U8) :
   ∃ new_a, adc_for_add_with_carry_back a b carry = .ret new_a ∧
-  new_a = (a.val + b.val + carry.val) * 2 ^ 64 := by sorry
+  new_a = (a.val + b.val + carry.val) % 2 ^ 64 := by sorry
 
 
-lemma add_with_carry_overflow : 
+lemma add_with_carry_overflow [Inhabited U64] : 
   ∀ (N : Usize) (self : arithmetics.BigInt N) (other : arithmetics.BigInt N),
   ∃ b, arithmetics.BigInt.add_with_carry N self other = .ret b ∧
   ¬b ↔ self.val + other.val ≤ BigInt.max_value N := sorry
     -- by unfold arithmetics.BigInt.add_with_carry
 
-lemma add_with_carry_correct :
+lemma add_with_carry_correct [Inhabited U64] :
   ∀ (N : Usize) (self : arithmetics.BigInt N) (other : arithmetics.BigInt N),
   ∃ v, arithmetics.BigInt.add_with_carry_back N self other = .ret v ∧
-  v.val = (self.val + other.val) % (BigInt.max_value N) := sorry
+  v.val = (self.val + other.val) % (BigInt.max_value N) := by
+    simp [arithmetics.BigInt.add_with_carry_back]
+    intro N
+    if hx : N = 1#usize then
+      rw [hx]
+      intro self other
+      simp 
+      progress with Array.index_usize_spec as ⟨ i, hi ⟩
+      progress with Array.index_usize_spec as ⟨ i0, hi0 ⟩
+      progress with adc_for_add_with_carry_back_spec as ⟨ i1, hi1 ⟩
+      progress with Array.update_usize_spec as ⟨ a1, ha1 ⟩
+      simp [BigInt.val, BigInt.max_value]
+      have h_self_val : i = self.val := by simp [hi, BigInt.val]; unfold BigInt.valImpl; simp [tmp, *]; unfold BigInt.valImpl; simp [tmp, *];
+      have h_bi_1_val : ∀ (bi : arithmetics.BigInt 1#usize), BigInt.valImpl bi.num.val = (bi.num.val).index 0#usize.val  := by intros; simp [hi, BigInt.val]; unfold BigInt.valImpl; simp [tmp, *]; unfold BigInt.valImpl; simp [tmp, *];
+      simp [h_bi_1_val]
+      simp [ha1]
+      unfold BigInt.valImpl
+      simp []
+      sorry
+    else 
+    sorry
 
 end arithmetics
 
